Primitive_Matchers/No_Spoof.thy
@@ -26,7 +26,7 @@ section{*No Spoofing*}
     lemma[code_unfold]: "ipassmt_sanity_haswildcards (map_of ipassmt) \<longleftrightarrow> (\<forall> iface \<in> fst` set ipassmt. \<not> iface_is_wildcard iface)"
       by(simp add: ipassmt_sanity_haswildcards_def Map.dom_map_of_conv_image_fst)
 
-    value(code) "ipassmt_sanity_haswildcards (map_of [(Iface ''eth1.1017'', [(ipv4addr_of_dotdecimal (131,159,14,240), 28)])])"
+    value[code] "ipassmt_sanity_haswildcards (map_of [(Iface ''eth1.1017'', [(ipv4addr_of_dotdecimal (131,159,14,240), 28)])])"
 
   fun collect_ifaces :: "common_primitive rule list \<Rightarrow> iface list" where
     "collect_ifaces [] = []" |
@@ -41,7 +41,7 @@ section{*No Spoofing*}
     lemma[code]: "ipassmt_sanity_defined rs ipassmt \<longleftrightarrow> (\<forall> iface \<in> set (collect_ifaces rs). ipassmt iface \<noteq> None)"
       by(simp add: ipassmt_sanity_defined_def Map.domIff)
   
-    value(code) "ipassmt_sanity_defined [Rule (MatchAnd (Match (Src (Ip4AddrNetmask (192,168,0,0) 24))) (Match (IIface (Iface ''eth1.1017'')))) action.Accept,
+    value[code] "ipassmt_sanity_defined [Rule (MatchAnd (Match (Src (Ip4AddrNetmask (192,168,0,0) 24))) (Match (IIface (Iface ''eth1.1017'')))) action.Accept,
              Rule (MatchAnd (Match (Src (Ip4AddrNetmask (192,168,0,0) 24))) (Match (IIface (ifaceAny)))) action.Accept,
              Rule MatchAny action.Drop]
              (map_of [(Iface ''eth1.1017'', [(ipv4addr_of_dotdecimal (131,159,14,240), 28)])])"
@@ -191,7 +191,7 @@ begin
                 {}"
 
   (*when we replace the set by a 32 wordinterval, we should get executable code*)
-  value(code) "primitive_extractor (is_Src, src_sel) (MatchAnd (Match (Src (Ip4AddrNetmask (0,0,0,0) 30))) (Match (IIface (Iface ''eth0''))))"
+  value[code] "primitive_extractor (is_Src, src_sel) (MatchAnd (Match (Src (Ip4AddrNetmask (0,0,0,0) 30))) (Match (IIface (Iface ''eth0''))))"
 
   private lemma match_simplematcher_Src_getPos: "(\<forall>m\<in>set (map Src (getPos ip_matches)). matches (common_matcher, \<alpha>) (Match m) a p)
          \<longleftrightarrow> (\<forall>ip\<in>set (getPos ip_matches). p_src p \<in> ipv4s_to_set ip)"
@@ -447,7 +447,7 @@ begin
       apply(simp_all add: NegPos_set)
     using NegPos_set(2) by fastforce
 
-  value(code) "(get_exists_matching_src_ips_executable (Iface ''eth0'')
+  value[code] "(get_exists_matching_src_ips_executable (Iface ''eth0'')
       (MatchAnd (MatchNot (Match (Src (Ip4AddrNetmask (192,168,0,0) 24)))) (Match (IIface (Iface ''eth0'')))))"
 
   private definition get_all_matching_src_ips_executable :: "iface \<Rightarrow> common_primitive match_expr \<Rightarrow> 32 wordinterval" where
@@ -495,7 +495,7 @@ begin
     apply(erule_tac x="Neg aa" in ballE)
      apply(simp_all add: NegPos_set)
     done
-  value(code) "(get_all_matching_src_ips_executable (Iface ''eth0'')
+  value[code] "(get_all_matching_src_ips_executable (Iface ''eth0'')
       (MatchAnd (MatchNot (Match (Src (Ip4AddrNetmask (192,168,0,0) 24)))) (Match (IIface (Iface ''eth0'')))))"
 
 
@@ -1142,12 +1142,12 @@ begin
 end
 
 
-value(code) "no_spoofing_iface (Iface ''eth1.1011'') ([Iface ''eth1.1011'' \<mapsto> [(ipv4addr_of_dotdecimal (131,159,14,0), 24)]]:: ipassignment)
+value[code] "no_spoofing_iface (Iface ''eth1.1011'') ([Iface ''eth1.1011'' \<mapsto> [(ipv4addr_of_dotdecimal (131,159,14,0), 24)]]:: ipassignment)
   [Rule (MatchNot (Match (IIface (Iface ''eth1.1011+'')))) action.Accept,
            Rule (MatchAnd (MatchNot (Match (Src (Ip4AddrNetmask (131,159,14,0) 24)))) (Match (IIface (Iface ''eth1.101'')))) action.Drop,
            Rule MatchAny action.Accept]"
 
-value(code) "no_spoofing_iface (Iface ''eth1.1011'') ([Iface ''eth1.1011'' \<mapsto> [(ipv4addr_of_dotdecimal (131,159,14,0), 24)]]:: ipassignment)
+value[code] "no_spoofing_iface (Iface ''eth1.1011'') ([Iface ''eth1.1011'' \<mapsto> [(ipv4addr_of_dotdecimal (131,159,14,0), 24)]]:: ipassignment)
   [Rule (Match (Src (Ip4AddrNetmask (127, 0, 0, 0) 8))) Drop]"
 
 
